# 14.3: Partial Derivatives

## Definition
If the limit exists, the **partial derivative** of $f(x, y)$ with respect to $x$ at $(x_0, y_0)$ is:
$$
\Large
\left.\frac{\partial{f}}{\partial{x}}\right|_{(x_0, y_0)} = \lim_{\Delta x \to 0} \frac{f(x_0 + \Delta x, y_0) - f(x, y)}{\Delta x}
$$
(Differentiate $f$ with respect to $x$, while holding other variables constant)
(This extends trivially to other variables & more dimensions)

## Differentiability
Function $z = f(x, y)$ is **differentiable** at $(x_0, y_0)$ if $f_x, f_y$ (the partial derivatives) and $\Delta z = f(x_0 + \Delta x, y_0 + \Delta y) - f(x_0, y_0)$ satisfies:
$$
\Large
\Delta z = (f_x + \epsilon_1)\Delta x + (f_y + \epsilon_2)\Delta y
$$
(where each $\epsilon_1, \epsilon_2 \to 0$ as both $\Delta x, \Delta y \to 0$)

$f$ is **differentiable** if it is differentiable at every point in its domain.
If $f$ is differentiable, then the graph of $f$ is called a **smooth surface**

**Why?**
In single variable calculus, given a function $y = f(x)$, the change in $\Delta y = f(x_0 + \Delta x) - f(x_0)$ can be approximated by the change according to the tangent line at that point.

$$
\Large
\begin{align*}
y - f(x_0) &= f'(x_0)(x - x_0) \text{ (tangent line form)}\\
f_{approx}(x_0 + \Delta x) - f(x_0) &= f'(x_0)\Delta x\\
\Delta y &\approx f'(x_0)\Delta x
\end{align*}
$$
If we let the difference in the correct slope $\epsilon$, $\Delta y = (f'(x_0) + \epsilon)\Delta x$.
(As $\Delta x \to 0, \epsilon \to 0$.)

Hence, we can extend this into multiple variables with multiple $\epsilon$.

### Example
Find all first partial derivatives of $f(x, y) = 3x^2 - 2y + xy$.
$$
\Large
\begin{align*}
f_x = \frac{\partial{f}}{\partial{x}} &= 6x + y\\
f_y = \frac{\partial{f}}{\partial{y}} &= -2 + x
\end{align*}
$$

## Second Order Partial Derivatives
$$
\Large
\begin{align*}
(f_x)_x = f_{xx} &= \frac{\partial}{\partial{x}}\left(\frac{\partial{f}}{\partial{x}}\right) = \frac{\partial^{2}{f}}{\partial{x^2}}\\
(f_x)_y = f_{xy} &= \frac{\partial}{\partial{y}}\left(\frac{\partial{f}}{\partial{x}}\right) = \frac{\partial^{2}{f}}{\partial{y}\partial{x}}\\
(f_y)_x = f_{yx} &= \frac{\partial}{\partial{x}}\left(\frac{\partial{f}}{\partial{y}}\right) = \frac{\partial^{2}{f}}{\partial{x}\partial{y}}\\
(f_y)_y = f_{yy} &= \frac{\partial}{\partial{y}}\left(\frac{\partial{f}}{\partial{y}}\right) = \frac{\partial^{2}{f}}{\partial{y^2}}\\
\end{align*}
$$
### Mixed Derivatives Theorem
If $f(x,y)$ and all of $\Large f_x, f_y, f_{xy}, f_{yx}$ are defined throughout an open region containing a point $(x_0, y_0)$ and are all continuous at $(x_0, y_0)$, then 
$$
\Large f_{xy}(x_0, y_0) = f_{yx}(x_0, y_0)
$$

### Example
Find all first & second partial derivatives of $f(x, y) = 2x^2\cos{y} + 3y^2\sin{x}$.

$$
\Large
\begin{align*}
f_x &= 4x\cos{y} + 3y^2\cos{x}\\
f_y &= -2x^2\sin{y} + 6y\sin{x}\\
\end{align*}
$$

$$
\Large
\begin{align*}
f_{xx} &= 4\cos{y} - 3y^2\sin{x}\\
f_{xy} &= -4x\sin{y} + 6y\cos{x}\\
f_{yx} &= -4x\sin{y} + 6y\cos{x}\\
f_{yy} &= -2x^2\cos{y} + 6\sin{x}
\end{align*}
$$

## Implicit Differentiation
Suppose we have a function in terms of three variables $x, y, z$ and we cannot solve the equation for $z$, but we want to find $\frac{\partial{z}}{\partial{x}}$ or $\frac{\partial{z}}{\partial{y}}$.

Do implicit differentiation as expected, but hold the necessary variables constant.

### Example
Find $\Large \frac{\partial{z}}{\partial{x}}$ and $\Large \frac{\partial{z}}{\partial{y}}$ for $\Large xy - z^2y - 2zx = 0$.

$$
\Large
\begin{align*}
y - 2zy\frac{\partial{z}}{\partial{x}} - 2z - 2x\frac{\partial{z}}{\partial{x}} &= 0 \\
\frac{\partial{z}}{\partial{x}}(-2zy - 2x) + y - 2z &= 0 \\
\frac{\partial{z}}{\partial{x}}(-2zy - 2x) &= 2z - y \\
\frac{\partial{z}}{\partial{x}} &= \frac{y - 2z}{2zy + 2x} \\
\end{align*}
$$

$$
\Large
\begin{align*}
x - z^2 - 2zy\frac{\partial{z}}{\partial{y}} - 2x\frac{\partial{z}}{\partial{y}} &= 0 \\
x - z^2 - (2zy+2x)\frac{\partial{z}}{\partial{y}} &= 0 \\
(2zy+2x)\frac{\partial{z}}{\partial{y}} &= x - z^2 \\
\frac{\partial{z}}{\partial{y}} &= \frac{x - z^2}{2zy+2x} \\
\end{align*}
$$

# 14.4: Chain Rule
## $\large x, y$ as functions of one variable
If $w = f(x, y)$ is differentiable and $x(t), y(t)$ are differentiable with respect to $t$, then $w = f(x(t), y(t))$ is differentiable with respect to $t$.
$$
\Large
\frac{dw}{dt} = \frac{\partial{w}}{\partial{x}}\frac{dx}{dt} + \frac{\partial{w}}{\partial{y}}\frac{dy}{dt}
$$
(This is trivially extendible to more dimensions)

### Example
Find $\Large \frac{du}{dt}: u = x^2 - 3xy = 2y^2,\text{ } x(t) = \cos{t},\text{ } y(t) = \sin{t}$

$$
\Large
\begin{align*}
\frac{dx}{dt} &= -\sin{t}\\
\frac{dy}{dt} &= \cos{t}\\
\frac{\partial{u}}{\partial{x}} &= 2x - 3y\\
\frac{\partial{u}}{\partial{y}} &= -3x + 4y\\
\end{align*}
$$
So:
$$
\Large
\begin{align*}
\frac{du}{dt} &= \frac{\partial{u}}{\partial{x}}\frac{dx}{dt} + \frac{\partial{u}}{\partial{y}}\frac{dy}{dt}\\\\
&= (2\cos(t) - 3\sin(t))(-\sin(t))\\
&\hspace{1.5em} + (-3\cos(t) + 4\sin(t))(\cos(t))\\\\
&= -2\sin(t)\cos(t) + 3\sin^2(t) - 3\cos^2(t) + 4\sin(t)\cos(t)\\
&= 2\sin(t)\cos(t) + 3\sin^2(t) - 3\cos^2(t)\\
&= \sin(2t) - 3\cos(2t)
\end{align*}
$$

## $\large x, y$ as functions of multiple variables
What if $u = u(x, y)$, $x = x(s, t)$, $y = y(s, t)$?

You can find partial derivatives $\Large \frac{\partial{u}}{\partial{s}}$ and $\Large \frac{\partial{u}}{\partial{t}}$, replacing $\Large \frac{dx}{dt}$ in the simpler chain rule with the respective partial derivative.
$$
\Large
\begin{align*}
\frac{\partial u}{\partial s} &= \frac{\partial{u}}{\partial{x}}\frac{\partial x}{\partial s} + \frac{\partial{u}}{\partial{y}}\frac{\partial y}{\partial s}\\
\frac{\partial u}{\partial t} &= \frac{\partial{u}}{\partial{x}}\frac{\partial x}{\partial t} + \frac{\partial{u}}{\partial{y}}\frac{\partial y}{\partial t}
\end{align*}
$$
#### Example
Given $z = 4e^x\ln{y}, x = \ln(uv), y = u\sin(v)$, express $\frac{\partial{z}}{\partial{u}}$ as a function of $u$ and $v$.

$$
\Large
\begin{align*}
\frac{\partial{x}}{\partial{u}} &= \frac{1}{u}\\
\frac{\partial{y}}{\partial{u}} &= \sin(v)\\\\
\frac{\partial{z}}{\partial{x}} &= 4e^x\ln{y} \\
&= 4uv\ln(u\sin(v))\\\\
\frac{\partial{z}}{\partial{y}} &= \frac{4e^x}{y} \\
&= \frac{4v}{\sin(v)}\\
\end{align*}
$$
So:
$$
\Large
\begin{align*}
\frac{\partial{z}}{\partial{s}} &= \frac{\partial{z}}{\partial{x}}\frac{\partial{x}}{\partial{u}} + \frac{\partial{z}}{\partial{y}}\frac{\partial{y}}{\partial{u}}\\\\
&= 4uv\ln(u\sin(v))\frac{1}{u} + \frac{4v}{\sin(v)}\sin(v)\\
&= 4v\ln(u\sin(v)) + 4v
\end{align*}
$$

## Implicit Differentiation (again)
If $F(x, y)$ is differentiable and $F(x, y) = 0$ defines $y$ as differentiable function of $x$,
$$
\Large
\frac{dy}{dx} = -\frac{F_x}{F_y}
$$
In 3D,
If $z = z(x, y)$ and $F(x, y, z(x, y)) = 0$, you can do the same thing, but to find $\frac{\partial{z}}{\partial{x}}, \frac{\partial{z}}{\partial{y}}$

**Why?**
Let $F$ be written as $F(x, y(x))$.
$$
\Large
\begin{align*}
F(x, y(x)) &= 0\\
\frac{d}{dx} F(x, y(x)) &= \frac{d}{dx}0\\
\frac{\partial{F}}{\partial{x}}\frac{dx}{dx} + \frac{\partial{F}}{\partial{y}}\frac{dy}{dx}&= 0\\
\frac{\partial{F}}{\partial{x}} + \frac{\partial{F}}{\partial{y}}\frac{dy}{dx}&= 0\\
F_x + F_y\frac{dy}{dx}&= 0\\
\frac{dy}{dx} = -\frac{F_x}{F_y}
\end{align*}
$$
### Examples
![[Pasted image 20220116112825.png]]
![[Pasted image 20220116113020.png]]

#module2 #week4